post.dfy
@@ -38,11 +38,11 @@ module PostOffice {
 		requires s.Time < 997
 
 		ensures s'.BoxCount == s.BoxCount + 1
-		// ensures s.Called ==> s'.Called
 		ensures if (s.BoxCount + 1 > 20 && !s.Called) 
 			then s'.Called && s'.CalledAt == s'.Time 
 			else s'.Called == s.Called && s'.CalledAt == s.CalledAt
 		ensures s'.Time == s.Time
+		ensures s'.BoxCount > 0
 		ensures Valid(s')
 	{
 		s' := s.(BoxCount := s.BoxCount + 1);
@@ -74,35 +74,31 @@ module PostOffice {
 		requires Valid(s)
 		requires s.Time < 1000 - 3
 		requires s.Called && s.Time - s.CalledAt == 2 ==> pick
-		requires pick ==> s.Called
-		requires pick ==> s.BoxCount > 0
 		requires pick ==> s.Called && s.BoxCount > 0
-		
+		requires s.Called ==> s.BoxCount > 0;
+
 		ensures s'.CalledAt < s'.Time
+		ensures s.Called ==> s'.CalledAt == s.CalledAt
 		ensures s'.Time <= 1000 - 3
 		ensures s'.Time == s.Time + 1
-		ensures (s'.Called ==> (s'.Time - s'.CalledAt <= 2))
-		// ensures drop && (if (s.BoxCount + 1 > 20 && !s.Called) 
-		// 	then s'.Called && s'.CalledAt == s'.Time 
-		// 	else s'.Called == s.Called && s'.CalledAt == s.CalledAt)
+		ensures if pick then s'.BoxCount == 0 else s'.BoxCount >= s.BoxCount
+		ensures if pick then !s'.Called else s.Called ==> s'.Called
+		ensures s'.Called ==> s'.BoxCount > 0
+		ensures s'.Called && !s.Called ==> s'.CalledAt == s.Time
 		ensures Valid(s')
 	{
 		s' := s;
 		if drop {
 			s' := DropOff(s');
-			assert (s'.Called ==> (s'.Time - s'.CalledAt <= 2));
-			// assert(if (s.BoxCount + 1 > 20 && !s.Called) 
-			// then s'.Called && s'.CalledAt == s'.Time 
-			// else s'.Called == s.Called && s'.CalledAt == s.CalledAt);
 		}
 		
 		if pick {
 			s' := PickUp(s');
-			assert (s'.Called ==> (s'.Time - s'.CalledAt == 2));
 		}
-		assert (s'.Called ==> (s'.Time - s'.CalledAt <= 2));
+
+		assert s'.Called ==> s'.BoxCount > 0;
 		s' := s'.(Time := s'.Time + 1);
-		
+		assert s'.Called ==> s'.BoxCount > 0;
 	}
 
 	// When finishing up the day
@@ -117,11 +113,13 @@ module PostOffice {
 		ensures s'.CalledAt < s'.Time
 		ensures 1000 - 3 < s'.Time <= 1000
 		ensures s'.Time == s.Time + 1
+		ensures s'.CalledAt == s.CalledAt
+		ensures if pick then s'.BoxCount == 0 else s'.BoxCount == s.BoxCount
+		ensures if pick then !s'.Called else s.Called == s'.Called
 		ensures Valid(s')
 	{
 		s' := s;
 		if pick {
-			assert s'.Called == true;
 			s' := PickUp(s');
 		}
 		s' := s'.(Time := s'.Time + 1);
@@ -140,44 +138,76 @@ module PostOffice {
 			invariant s.Called ==> (0 < s.Time - s.CalledAt <= 2)
 
 			invariant 0 <= s.Time <= 1000 - 1
+			invariant s.Time > 1000 - 2 ==> s.BoxCount == 0
 			invariant |pickups| == 2
 			invariant old(|dropoffs|) == |dropoffs|
+			invariant (s.Called && s.CalledAt == s.Time - 1) == pickups[1]
+			invariant (s.Called && s.CalledAt == s.Time - 2) ==> pickups[0]
+			invariant s.Called ==> true in pickups
+			invariant s.Called ==> s.BoxCount > 0		
+			invariant pickups[0] ==> !pickups[1]
+			invariant pickups[1] ==> !pickups[0]
+			invariant pickups[0] ==> s.BoxCount > 0 && s.Called
 			invariant s.BoxCount > 0 && s.Time == 1000 - 3 ==> s.Called
 			invariant s.BoxCount > 0 && s.Time == 1000 - 3 ==> true in pickups
 			invariant s.BoxCount > 0 && s.Time == 1000 - 2 ==> true in pickups[..(|pickups|-1)]
 		{
 			var stime_old := s.Time;
 			var pickups_old := pickups;
-			var calledat_old := s.CalledAt;
+			var scalledat_old := s.CalledAt;
 			var scalled_old := s.Called;
-			assert s.Called && s.CalledAt == stime_old - 2 ==> pickups[0];
+			var sboxcount_old := s.BoxCount;
+
 			if s.Time < 1000 - 3 {
 				s := TickMidday(dropoffs[s.Time], pickups[0], s);
-				assume scalled_old && s.CalledAt == calledat_old; // TODO
-				assert scalled_old ==> s.CalledAt == calledat_old;
+				assert pickups_old[0] == pickups[0];
+				assert !pickups_old[0] ==> scalled_old ==> s.Called;
 			} else {
-				assert s.BoxCount > 0 ==> pickups[0] || pickups[1];
 				s := TickEoD(pickups[0], s);
 			}
+
+			assert scalled_old ==> s.CalledAt == scalledat_old;
+			
 			if s.Time == 1000 - 3 {
 				if s.BoxCount > 0 && !s.Called {
 					s := s.(Called := true, CalledAt := s.Time - 1); // -1 since already incremented by now
 				}
 			}
-			assume scalled_old ==> !s.Called;
-			assert scalled_old ==> s.CalledAt == calledat_old;
-			pickups := pickups[1..] + [s.Called && s.CalledAt == s.Time - 1];
 
+			assert scalled_old ==> s.CalledAt == scalledat_old;
+			assert !pickups_old[0] ==> s.BoxCount >= sboxcount_old;
+
+			pickups := pickups[1..] + [s.Called && s.CalledAt == s.Time - 1];
+			
+			assert pickups[0] ==> s.Called;
+			assert s.Called ==> s.BoxCount > 0;
+			assert pickups[0] ==> s.BoxCount > 0;
+			assert pickups[0] ==> s.BoxCount > 0 && s.Called;
+			assert pickups[1] ==> s.BoxCount > 0;
+
+			//proof of s.BoxCount > 0 && s.Time == 1000 - 3 ==> true in pickups
 			assert s.Called ==> (s.Time - s.CalledAt == 1 || s.Time - s.CalledAt == 2);
-			assert (scalled_old && calledat_old == stime_old - 1 ==> pickups_old[1]) ==> scalled_old == s.Called;
-			assert scalled_old ==> s.CalledAt == calledat_old;
 			assert pickups_old[1] == pickups[0];
 			assert stime_old == s.Time - 1;
-			assert scalled_old && calledat_old == stime_old - 1 ==> pickups_old[1];
-			
-			assert s.Called && s.CalledAt == s.Time - 2 ==> pickups[0];
-			assert s.Called && s.CalledAt == s.Time - 1 ==> pickups[1];
+			assert pickups_old[1] ==> !pickups_old[0];
+			assert !pickups_old[0] ==> scalled_old ==> s.Called;
+			assert scalled_old && scalledat_old == stime_old - 1 ==> s.Called;
+			assert (scalled_old && scalledat_old == stime_old - 1) == pickups_old[1];
+			assert scalled_old && scalledat_old == stime_old - 1 ==> scalled_old == s.Called;			
+
+			assert s.Called && s.Time - s.CalledAt == 2 ==> scalled_old;
+			assert (s.Called && s.CalledAt == s.Time - 2) ==> (scalled_old && scalledat_old == stime_old - 1);
+			assert (s.Called && s.CalledAt == s.Time - 2) ==> pickups[0];
+			assert (s.Called && s.CalledAt == s.Time - 1) == pickups[1];
 			assert s.Called ==> true in pickups;
+
+			//proof of s.BoxCount > 0 && s.Time == 1000 - 2 ==> true in pickups[..(|pickups|-1)]
+			assert stime_old == 997 && sboxcount_old > 0 ==> scalled_old;
+			assert s.Time == 998 && s.BoxCount > 0 ==> sboxcount_old > 0;
+			assert s.Time == 998 && s.BoxCount > 0 ==> scalled_old;
+			assert s.Time == 998 && s.BoxCount > 0 ==> (scalled_old && scalledat_old == stime_old - 1);
+			assert s.Time == 998 && s.BoxCount > 0 ==> pickups_old[1];
+			assert s.Time == 998 && s.BoxCount > 0 ==> pickups[0];
 		}
 		assert (s.Time == 1000 - 1);
 		assert (s.BoxCount == 0);
